Updated ProcStep and EnvStep

PiLL/PiLL/Framework/Semantics/EnvStep.lean
@@ -3,20 +3,20 @@ import PiLL.Framework.Semantics.Labels
 
 inductive EnvStep : HyperEnv → Lbl → HyperEnv → Prop where
   | one
-      {x : PName} :
-      EnvStep (x ∶ 1) (x⟦⟧) ∅
+      {x : FPName} :
+      EnvStep [[x ∶ 1]] (x⟦⟧) ∅
 
   | tensor
-      {Γ Δ : Env} {x x' : PName} {A B : Types} :
-      EnvStep (Γ‚ Δ‚ x ∶ A ⨂ B) (x⟦x'⟧) (Γ‚ x'∶ A |ₕ Δ‚ x ∶ B)
+      {Γ Δ : Env} {x x' : FPName} {A B : Types} :
+      EnvStep [x ∶ A ⨂ B :: Γ‚ Δ] (x⟦x'⟧) ([x'∶ A :: Γ] |ₕ [x ∶ B :: Δ])
 
   | bot
-      {Γ : Env} {x : PName} :
-      EnvStep (Γ‚ x ∶ ⊥) (x⸨⸩) Γ
+      {Γ : Env} {x : FPName} :
+      EnvStep [x ∶ ⊥ :: Γ] (x⸨⸩) [Γ]
 
   | parr
-      {Γ Δ : Env} {x x' : PName} {A B : Types} :
-      EnvStep (Γ‚ x ∶ A ⅋ B) (x⸨x'⸩) (Γ‚ x' ∶ A‚ Δ‚ x ∶ B)
+      {Γ : Env} {x x' : FPName} {A B : Types} :
+      EnvStep [x ∶ A ⅋ B :: Γ] (x⸨x'⸩) [x ∶ B :: x' ∶ A :: Γ]
 
   | par₁
       {𝒢 𝒢' ℋ : HyperEnv} {l : Lbl} :
@@ -37,85 +37,81 @@ inductive EnvStep : HyperEnv → Lbl → HyperEnv → Prop where
       EnvStep (𝒢 |ₕ ℋ) (l |ₗ l') (𝒢' |ₕ ℋ')
 
   | one_bot
-      {𝒢 : HyperEnv} {Γ : Env} {x y : PName} :
-      EnvStep (𝒢 |ₕ x ∶ 1 |ₕ Γ‚ y ∶ ⊥) (x⟦⟧ |ₗ y⸨⸩) (𝒢 |ₕ Γ) →
-      ------------------------------------------------------
-      EnvStep (𝒢 |ₕ Γ) (τ) (𝒢 |ₕ Γ)
+      {𝒢 : HyperEnv} {Γ : Env} {x y : FPName} :
+      EnvStep (𝒢 |ₕ [[x ∶ 1]] |ₕ [y ∶ ⊥ :: Γ]) (x⟦⟧ |ₗ y⸨⸩) (𝒢 |ₕ [Γ]) →
+      ---------------------------------------------------------------
+      EnvStep (𝒢 |ₕ [Γ]) (τ) (𝒢 |ₕ [Γ])
 
   | tensor_parr
-      {𝒢 : HyperEnv} {Γ Δ Ξ : Env} {x x' y y': PName} {A B : Types} :
+      {𝒢 : HyperEnv} {Γ Δ Ξ : Env} {x x' y y': FPName} {A B : Types} :
       EnvStep
-        (𝒢 |ₕ Γ‚ Δ‚ x ∶ A ⨂ B |ₕ Ξ‚ y ∶ Aᗮ ⅋ Bᗮ)
+        (𝒢 |ₕ [x ∶ A ⨂ B :: Γ‚ Δ] |ₕ [y ∶ Aᗮ ⅋ Bᗮ :: Ξ])
         (x⟦x'⟧ |ₗ y⸨y'⸩)
-        (𝒢 |ₕ Γ‚ x' ∶ A |ₕ Δ‚ x ∶ B |ₕ Ξ‚ y' ∶ Aᗮ‚ y ∶ Bᗮ) →
-      ---------------------------------------------------
-      EnvStep (𝒢 |ₕ Γ‚ Δ‚ Ξ) (τ) (𝒢 |ₕ Γ‚ Δ‚ Ξ)
+        (𝒢 |ₕ [x' ∶ A :: Γ] |ₕ [x' ∶ A :: Δ] |ₕ [y ∶ Bᗮ :: y' ∶ Aᗮ :: Ξ]) →
+      ------------------------------------------------------------------
+      EnvStep (𝒢 |ₕ [Γ‚ Δ‚ Ξ]) (τ) (𝒢 |ₕ [Γ‚ Δ‚ Ξ])
 
   | res
-      {𝒢 𝒢' : HyperEnv} {Γ Γ' Δ Δ' : Env} {x y : PName} {A B : Types} {l : Lbl} :
-      EnvStep (𝒢 |ₕ Γ‚ x ∶ Aᗮ |ₕ Δ‚ y ∶ A) (l) (𝒢' |ₕ Γ'‚ x ∶ Aᗮ |ₕ Δ'‚ y ∶ A) →
-      ----------------------------------------------------------------------------
-      EnvStep (𝒢 |ₕ Γ‚ Δ) l (𝒢' |ₕ Γ'‚ Δ')
+      {𝒢 𝒢' : HyperEnv} {Γ Γ' Δ Δ' : Env} {x y : FPName} {A B : Types} {l : Lbl} :
+      EnvStep (𝒢 |ₕ [x ∶ Aᗮ :: Γ] |ₕ [y ∶ A :: Δ]) (l) (𝒢' |ₕ [x ∶ Aᗮ :: Γ'] |ₕ [y ∶ A :: Δ']) →
+      -------------------------------------------------------------------------------------
+      EnvStep (𝒢 |ₕ [Γ‚ Δ]) l (𝒢' |ₕ [Γ'‚ Δ'])
 
   | selectL
-      {Γ : Env} {x : PName} {A B : Types} :
-      EnvStep (Γ‚ x ∶ A ⊕ B) (x⟦𝐋⟧) (Γ‚ x ∶ A)
+      {Γ : Env} {x : FPName} {A B : Types} :
+      EnvStep [x ∶ A ⊕ B :: Γ] (x⟦𝐋⟧) [x ∶ A :: Γ]
 
   | ampL
-      {Γ : Env} {x : PName} {A B : Types} :
-      EnvStep (Γ‚ x ∶ A & B) (x⸨𝐋⸩) (Γ‚ x ∶ A)
+      {Γ : Env} {x : FPName} {A B : Types} :
+      EnvStep [x ∶ A & B :: Γ] (x⸨𝐋⸩) [x ∶ A :: Γ]
 
   | selectR
-      {Γ : Env} {x : PName} {A B : Types} :
-      EnvStep (Γ‚ x ∶ A ⊕ B) (x⟦𝐑⟧) (Γ‚ x ∶ B)
+      {Γ : Env} {x : FPName} {A B : Types} :
+      EnvStep [x ∶ A ⊕ B :: Γ] (x⟦𝐑⟧) [x ∶ B :: Γ]
 
   | ampR
-      {Γ : Env} {x : PName} {A B : Types} :
-      EnvStep (Γ‚ x ∶ A & B) (x⸨𝐑⸩) (Γ‚ x ∶ B)
+      {Γ : Env} {x : FPName} {A B : Types} :
+      EnvStep [x ∶ A & B :: Γ] (x⸨𝐑⸩) [x ∶ B :: Γ]
 
   | link₁
-      {x y : PName} {A : Types} :
-      EnvStep (x ∶ Aᗮ‚ y ∶ A) (x ⟷ₗ y) ∅
-
---   | link₂ -- FIXME this one isn't actually in the definition in Fig 8, but it matches ProcStep
---       {x y : PName} {A : Types} :
---       EnvStep (x ∶ Aᗮ‚ y ∶ A) (y ⟷ₗ x) ∅
+      {x y : FPName} {A : Types} :
+      EnvStep [x ∶ Aᗮ :: [y ∶ A]] (x ⟷ₗ y) ∅
 
   | use₁
-      {Γ : Env} {x : PName} {A : Types} :
-      EnvStep (Γ‚ x ∶ ??A) (x⟦USE⟧) (Γ‚ x ∶ A)
+      {Γ : Env} {x : FPName} {A : Types} :
+      EnvStep [x ∶ ??A :: Γ] (x⟦USE⟧) [x ∶ A :: Γ]
 
   | use₂
-      {Γ : Env} {x : PName} {A : Types} :
+      {Γ : Env} {x : FPName} {A : Types} :
       ?ₑΓ →
-      --------------------------------------
-      EnvStep (Γ‚ x ∶ !!A) (x⸨USE⸩) (Γ‚ x ∶ A)
+      -------------------------------------------
+      EnvStep [x ∶ !!A :: Γ] (x⸨USE⸩) [x ∶ A :: Γ]
 
   | disp₁
-      {Γ : Env} {x : PName} {A : Types} :
-      EnvStep (Γ‚ x ∶ ??A) (x⟦DISP⟧) (Γ‚ x ∶ ⊥)
+      {Γ : Env} {x : FPName} {A : Types} :
+      EnvStep [x ∶ ??A :: Γ] (x⟦DISP⟧) [x ∶ ⊥ :: Γ]
 
   | disp₂
-      {Γ : Env} {x : PName} {A : Types} :
-      EnvStep {Γ‚ x ∶ !!A} (x⸨DISP⸩) (Γ‚ x ∶ 1)
+      {Γ : Env} {x : FPName} {A : Types} :
+      EnvStep [x ∶ !!A :: Γ] (x⸨DISP⸩) [x ∶ 1 :: Γ]
 
   | dup₁
-      {Γ : Env} {x : PName} {A : Types} :
-      EnvStep (Γ‚ x ∶ ??A) (x⟦DUP⟧) (Γ‚ x ∶ ??A ⅋ ??A)
+      {Γ : Env} {x : FPName} {A : Types} :
+      EnvStep [x ∶ ??A:: Γ] (x⟦DUP⟧) [x ∶ ??A ⅋ ??A :: Γ]
 
   | dup₂
-      {Γ : Env} {x : PName} {A : Types} :
+      {Γ : Env} {x : FPName} {A : Types} :
       ?ₑΓ →
-      ----------------------------------------------
-      EnvStep (Γ‚ x ∶ !!A) (x⸨DUP⸩) (Γ‚ x ∶ !!A ⨂ !!A)
+      ---------------------------------------------------
+      EnvStep [x ∶ !!A :: Γ] (x⸨DUP⸩) [x ∶ !!A ⨂ !!A :: Γ]
 
   | output
-      {Γ : Env} {x : PName} {A B : Types} {X : TVar} :
-      EnvStep (Γ‚ x ∶ ∃X․B) (x⟦A⟧) (Γ‚ x ∶ B{A // X})
+      {Γ : Env} {x : FPName} {A B : Types} {X : TVar} :
+      EnvStep [x ∶ ∃․B :: Γ] (x⟦A⟧) [x ∶ B{A // 0} :: Γ]
 
   | input
-      {Γ : Env} {x : PName} {A B : Types} {X : TVar} :
-      EnvStep (Γ‚ x ∶ ∀X․B) (x⸨A⸩) (Γ‚ x ∶ B{A // X})
+      {Γ : Env} {x : FPName} {A B : Types} {X : TVar} :
+      EnvStep [x ∶ ∀․B :: Γ] (x⸨A⸩) [x ∶ B{A // 0} :: Γ]
 
 notation:50 P " -[" l "]->ₑ " P' => EnvStep P l P'
 
