PiLL/PiLL/Framework/Semantics/SessionFidelity.lean
@@ -1,0 +1,92 @@
+import PiLL.Framework.Semantics.EnvStep
+import PiLL.Framework.Semantics.ProcStep
+
+
+
+-- FIXME: Fix TypingStep
+-- FIXME: Typing_preserves_proc_congr
+
+
+-- FIXME: Proof showing substitution avoids capture
+-- FIXME: Check possibility of no having exchange rules
+-- FIXME: Find different syntax for open?
+
+-- FIXME: Proof of HyperEnv.names only having free names
+-- FIXME: Proof that HyperEnv.names = Proc.f
+-- FIXME: Something regarding Name substitution only being applied to free names?
+
+
+-- NOTE: shows the proof lean found using the simp_all tactic show_term { simp_all }
+
+
+
+
+lemma typing_inv_one {n : ℕ} {P : Proc} {x : FPName} {𝒢 : HyperEnv}
+  (hT : Typing n (#x⟦⟧․P) 𝒢) :
+  (𝒢 ~ [[x ∶ 1]]) ∧ Typing n P ∅ := by
+  generalize heq : (#x⟦⟧․P) = P' at hT
+  induction hT generalizing P x <;> try contradiction
+
+  case exchange_env ih =>
+    have := ih (P := P) (x := x) heq
+    simp_all
+
+  case exchange_hyper ih =>
+    have := ih (P := P) (x := x)
+    simp at this
+    simp_all
+
+  case one hT _ =>
+    simp at heq
+    constructor
+    · simp [heq.1]
+    · simp [heq.2]
+      exact hT
+
+
+
+
+
+lemma EnvStep_equiv {𝒢 𝒢' ℋ : HyperEnv} {l : Lbl} :
+  EnvStep 𝒢 l 𝒢' → (𝒢 ~ ℋ) →
+  ∃ ℋ', EnvStep ℋ l ℋ' ∧ (𝒢' ~ ℋ') := by
+  intros hE
+  induction hE
+  case one | bot | selectL | selectR | ampL | ampR =>
+    intros h
+    simp_all
+    subst h
+    constructor
+
+  case input X | output X =>
+    intros h
+    simp_all
+    subst h
+    constructor
+    exact X
+
+  all_goals sorry
+
+
+
+
+
+
+
+
+
+
+
+-- FIXME: Subject reduction / simulation proof
+theorem session_fidelity {n : Nat} {P P' : Proc} {𝒢 : HyperEnv} {l : Lbl} :
+  Typing n P 𝒢 → ProcStep P l P' →
+  ∃ 𝒢', EnvStep 𝒢 l 𝒢' ∧ Typing n P' 𝒢' := by
+  intros hT hPS
+  induction hPS generalizing n 𝒢
+
+  case one =>
+    obtain ⟨hPerm, 𝒟⟩ := typing_inv_one hT
+
+
+
+  all_goals sorry
